$$\begin{aligned}
  \underset{x, y}{\text{minimize}}\qquad& \sum_{i\in A}\left(\sum_{t = 1}^{T} \sum_{j\in A} tx_{ij}^{t} - \sum_{t = 1}^{T} ty_{i}^{t} \right)\\
    \text{subject to:}\qquad& \sum_{t = 1}^{T} \sum_{j\in A} x_{ij}^{t} = 1 && \forall i \in A\\
    & \sum_{t = 1}^{T} \sum_{i \in A} x_{ij}^{t} = 1 && \forall j \in A \\
    & \sum_{t = 1}^{T} y_{i}^{t} = 1 && \forall i \in A \\
    & \sum_{i \in A} y_{i}^{t} \le 1 && \forall t \in \{ 1, \dots , T \}\\
    & \sum_{j\in A} x_{ij}^{t} \le \sum_{k = 0}^{t} y_{i}^{k} && \forall i \in A, \quad \forall t \in \{ 1, \dots , T \}\\
    & y_{i}^{t} w_{i}^{t} \le \gamma \sum_{j\in A} tx_{ij}^{t} - ty_{i}^{t} && \forall i \in A, \quad \forall t \in \{ 1, \dots , T \} \\
    & x_{ij}^{t} \in \{0, 1\} && \forall i,j \in A, \quad \forall t \in \{ 1, \dots , T \} \\
    & y_{i}^{t} \in \{0, 1\} && \forall i \in A, \quad \forall t \in \{ 1, \dots , T \}
\end{aligned}$$
